ImpHCons.v
@@ -12,37 +12,97 @@ Extract Constant string_of_hashcode => "string_of_int".
 Axiom hash: forall {A}, A -> ?? hashcode.
 Extract Constant hash => "Hashtbl.hash".
 
-Axiom xhCons: forall {A}, ((A -> A -> ?? bool) * (pre_hashV A -> ?? hashV A)) -> ?? hashConsing A.
+
+
+Module HConsing.
+
+Export HConsingDefs.
+
+(* NB: this axiom is NOT intended to be called directly, but only through [hCons...] functions below. *)
+Axiom xhCons: forall {A}, (hashH A) -> ?? hashConsing A.
 Extract Constant xhCons => "ImpHConsOracles.xhCons".
 
-Definition hCons_eq_msg: pstring := "xhCons: hash_eq differs".
+Definition hCons_eq_msg: pstring := "xhCons: hash eq differs".
 
-Definition hCons {A} (hash_eq: A -> A -> ?? bool) (unknownHash_msg: pre_hashV A -> ?? pstring): ?? (hashConsing A) :=
-  DO hco <~ xhCons (hash_eq, fun v => DO s <~ unknownHash_msg v ;; FAILWITH s) ;;
+Definition hCons {A} (hh: hashH A): ?? (hashConsing A) :=
+  DO hco <~ xhCons hh ;;
   RET {|
-      hC := fun x => 
-       DO x' <~ hC hco x ;;
-       DO b0 <~ hash_eq (pre_data x) (data x') ;;
-       assert_b b0 hCons_eq_msg;;
-       RET x';
-      hC_known := fun x => 
-       DO x' <~ hC_known hco x ;;
-       DO b0 <~ hash_eq (pre_data x) (data x') ;;
-       assert_b b0 hCons_eq_msg;;
-       RET x';
-      next_log := next_log hco;
-      export := export hco;
+      hC := (fun x =>
+         DO x' <~ hC hco x ;;
+         DO b0 <~ hash_eq hh x.(hdata) x' ;;
+         assert_b b0 hCons_eq_msg;;
+         RET x');
+      next_hid := hco.(next_hid);
+      next_log := hco.(next_log);
+      export := hco.(export);
+      remove := hco.(remove)
       |}.
 
-Lemma hCons_correct: forall A (hash_eq: A -> A -> ?? bool) msg,
-  WHEN hCons hash_eq msg ~> hco THEN
-    ((forall x y, WHEN hash_eq x y ~> b THEN b=true -> x=y) -> forall x, WHEN hC hco x ~> x' THEN (pre_data x)=(data x'))
- /\ ((forall x y, WHEN hash_eq x y ~> b THEN b=true -> x=y) -> forall x, WHEN hC_known hco x ~> x' THEN (pre_data x)=(data x')).
+
+Lemma hCons_correct A (hh: hashH A):
+  WHEN hCons hh ~> hco THEN
+    (forall x y, WHEN hh.(hash_eq) x y ~> b THEN b=true -> (ignore_hid hh x)=(ignore_hid hh y)) ->
+    forall x, WHEN hco.(hC) x ~> x' THEN ignore_hid hh x.(hdata)=ignore_hid hh x'.
 Proof.
   wlp_simplify.
 Qed.
 Global Opaque hCons.
 Hint Resolve hCons_correct: wlp.
 
-Definition hCons_spec {A} (hco: hashConsing A) :=
-  (forall x, WHEN hC hco x ~> x' THEN (pre_data x)=(data x')) /\ (forall x, WHEN hC_known hco x ~> x' THEN (pre_data x)=(data x')).
+
+
+(* hashV: extending a given type with hash-consing *)
+Record hashV {A:Type}:= {
+  data: A;
+  hid: hashcode
+}.
+Arguments hashV: clear implicits.
+
+Definition hashV_C {A} (test_eq: A -> A -> ?? bool) : hashH (hashV A) := {|
+  hash_eq := fun v1 v2 => test_eq v1.(data) v2.(data);
+  get_hid := hid;
+  set_hid := fun v id => {| data := v.(data); hid := id |}
+|}.
+
+Definition liftHV (x:nat) := {| data := x; hid := unknown_hid |}.
+
+Definition hConsV {A} (hasheq: A -> A -> ?? bool): ?? (hashConsing (hashV A)) :=
+  hCons (hashV_C hasheq).
+
+Lemma hConsV_correct A (hasheq: A -> A -> ?? bool):
+  WHEN hConsV hasheq ~> hco THEN
+    (forall x y, WHEN hasheq x y ~> b THEN b=true -> x=y) -> 
+    forall x, WHEN hco.(hC) x ~> x' THEN x.(hdata).(data)=x'.(data).
+Proof.
+  Local Hint Resolve f_equal2.
+  wlp_simplify.
+  exploit H; eauto.
+  + wlp_simplify.
+  + intros; congruence.
+Qed.
+Global Opaque hConsV.
+Hint Resolve hConsV_correct: wlp.
+
+Definition hC_known {A} (hco:hashConsing (hashV A)) (unknownHash_msg: hashinfo (hashV A) -> ?? pstring) (x:hashinfo (hashV A)): ?? hashV A :=
+  DO clock <~ hco.(next_hid)();;
+  DO x' <~ hco.(hC) x;;
+  DO ok <~ hash_older x'.(hid) clock;;
+  if ok 
+  then RET x'
+  else
+    hco.(remove) x;; 
+    DO msg <~ unknownHash_msg x;;
+    FAILWITH msg.
+
+Lemma hC_known_correct A (hco:hashConsing (hashV A)) msg x:
+  WHEN hC_known hco msg x ~> x' THEN
+    (forall x, WHEN hco.(hC) x ~> x' THEN x.(hdata).(data)=x'.(data)) ->
+    x.(hdata).(data)=x'.(data).
+Proof.
+  wlp_simplify.
+  unfold wlp in * |- ; eauto.
+Qed.
+Global Opaque hC_known.
+Hint Resolve hC_known_correct: wlp.
+
+End HConsing.
